work/container-overlay/polcert/driver/CPolOpt.v
@@ -7,11 +7,6 @@ Require Import ImpureAlarmConfig.
 Require Import Vpl.Impure.
 
 Module CoreOpt := PolOpt CPolIRs.
-Module TilingCheck := CoreOpt.TilingCheck.
-Module Tiling := CoreOpt.CheckedTiling.Tiling.
-Module TilingPolIRs := CoreOpt.CheckedTiling.TilingPolIRs.
-Module TilingVal := CoreOpt.CheckedTiling.TilingVal.
-Module TPrepare := CoreOpt.CheckedTiling.TPrepare.
 
 Definition opt : CPolIRs.Loop.t -> imp CPolIRs.Loop.t := CoreOpt.Opt.
 
