work/container-overlay/polcert/driver/TPolOpt.v
@@ -2,16 +2,13 @@ Require Import TPolIRs.
 Require Import OpenScop.
 Require Import Result.
 Require Import PolOpt.
+Require Import TilingRelation.
 Require Import TilingWitness.
 Require Import ImpureAlarmConfig.
 Require Import Vpl.Impure.
 
 Module CoreOpt := PolOpt TPolIRs.
-Module TilingCheck := CoreOpt.TilingCheck.
-Module Tiling := CoreOpt.CheckedTiling.Tiling.
-Module TilingPolIRs := CoreOpt.CheckedTiling.TilingPolIRs.
-Module TilingVal := CoreOpt.CheckedTiling.TilingVal.
-Module TPrepare := CoreOpt.CheckedTiling.TPrepare.
+Module Tiling := TilingRelation TPolIRs.Instr.
 
 Definition opt : TPolIRs.Loop.t -> imp TPolIRs.Loop.t := CoreOpt.Opt.
 
